src/coq/CompilerProp.v
@@ -12,11 +12,9 @@ Require Import Vellvm.Maps Vellvm.Imp.
 
 Require Import QuickChick.QuickChick.
 Import QcDefaultNotation. Open Scope qc_scope.
-Require Import List ZArith.
-Import ListNotations.
-Require Import String.
 
 Require Import ZArith String Omega List Equalities MSets.
+Import ListNotations.
 
 (* Vellvm dependencies *)
 Require Import Vellvm.Ollvm_ast Vellvm.Compiler Vellvm.AstLib Vellvm.CFG Vellvm.StepSemantics Vellvm.Memory.
@@ -58,31 +56,66 @@ Fixpoint imp_memory_eqb (m1 : list dvalue) (m2 : list dvalue) : bool :=
 Require Import List.
 
 
-Definition state_to_string (st : state) (fv : list id) : string :=
+
+
+Fixpoint string_of_dvalue' (v : value) :=
+  match v with
+  | DV expr =>
+    match expr with
+    | VALUE_Ident id => string_of id
+    | VALUE_Integer x => string_of x
+    | VALUE_Bool b => string_of b
+    | VALUE_Null => "null"
+    | VALUE_Zero_initializer => "zero initializer"
+    | VALUE_Cstring s => s
+    | VALUE_None => "none" 
+    | VALUE_Undef => "undef" 
+    | OP_IBinop iop t v1 v2 =>
+      ((string_of iop) ++ " " ++ (string_of t)
+                       ++ " " ++ (string_of_dvalue' v1)
+                       ++ " " ++ (string_of_dvalue' v2))%string
+    | OP_GetElementPtr t ptrval idxs =>
+      "getelementptr"
+    | _ => "string_of_dvalue' todo"
+    end
+  | DVALUE_CodePointer p => "string_of_dvalue' todo (code pointer)"
+  | DVALUE_Addr a => "string_of_dvalue' todo (addr)"
+  end.
+
+Instance string_of_value : StringOf dvalue := string_of_dvalue'.
+
+Instance string_of_mem : StringOf mtype :=
+  fun mem => ("[" ++ show_nat (List.length mem) ++ "] " ++ string_of mem)%string.
+(*
+  fun (mem: mtype) =>
+    fold_left (fun s cell =>
+                 match cell with
+                 | DV (VALUE_Integer z) => (s ++ (string_of z) ++ "; ")%string
+                 | DVALUE_CodePointer p => (s ++ "code pointer; ")%string
+                 | DVALUE_Addr a => (s ++ "addr; ")%string
+                 | _ => (s ++ "~VALUE_Integer; ")%string
+                 end)
+              mem "".
+*)
+
+Definition state_to_string (fv : list id) (st : state) : string :=
   fold_left (fun acc x => (match x with
                         | Id ident => (ident ++ ": " ++ show_nat (st x) ++ ", ")%string
                         end)) fv "".
 
-Check fold_left.
-Check show_int.
+Instance string_of_IDSet_elt : StringOf IDSet.elt :=
+  fun elem => 
+    match elem with
+    | Id name => name
+    end.
 
-Definition mem_to_string (mem : mtype) : string :=
-  fold_left (fun s cell =>
-               match cell with
-               | DV (VALUE_Integer z) => (s ++ (string_of z) ++ "; ")%string
-               | _ => (s ++ "~VALUE_Integer; ")%string
-               end)
-            mem "".
-
-Definition elt_to_string (elem : IDSet.elt) :=
-  match elem with
-  | Id name => name
-  end.
-
-Definition elems_to_string (elements : list IDSet.elt) : string :=
-  fold_left (fun s elem => (s ++ ", " ++ (elt_to_string elem)))%string
-            elements
-            "".
+(*
+Instance string_of_elems : StringOf (list IDSet.elt) :=
+  fun (elements : list IDSet.elt) =>
+    fold_left (fun s elem => (s ++ ", " ++ (string_of elem)))%string
+              elements
+              "".
+*)
 
 Definition imp_compiler_correct_aux (p:Imp.com) :=
   let fvs := IDSet.elements (fv p) in
@@ -97,7 +130,7 @@ Definition imp_compiler_correct_aux (p:Imp.com) :=
       | inl e => whenFail "init failed" false
       | inr initial_state =>
         let semantics := sem mcfg initial_state in
-        let llvm_final_state := MemDFin [] semantics 1000 in
+        let llvm_final_state := MemDFin [] semantics 10000 in
         let imp_state := ceval_step empty_state p 10000 in
         match (llvm_final_state, imp_state) with
         | (None, None) => whenFail "both out of gas" true
@@ -106,21 +139,18 @@ Definition imp_compiler_correct_aux (p:Imp.com) :=
         | (Some llvm_st, Some imp_st) => 
           let ans_state := List.map (fun x => dvalue_of_nat (imp_st x)) fvs in
           whenFail ("not equal: llvm: "
-                      ++ (mem_to_string llvm_st)
+                      ++ (string_of llvm_st)
                       ++ "; imp: "
-                      ++ (mem_to_string ans_state)
+                      ++ (string_of ans_state)
                       ++ "; free vars: "
-                      ++ (elems_to_string fvs))
+                      ++ (string_of fvs) (* (elems_to_string fvs) *)
+                      ++ "; compiled code: "
+                      ++ (string_of ll_prog))
                    (checker (imp_memory_eqb llvm_st ans_state))
         end        
       end
     end
   end.
-
-Example prog1 := W ::= AId W.
-Example prog2 := X ::= APlus (AId W) (AId W).
-
-Eval vm_compute in (compile prog2).
 
 
 
