src/coq/CompilerQuickChick.v
@@ -1,6 +1,8 @@
 
-Require Import Vellvm.Maps Vellvm.Imp Vellvm.CompilerProp.
+Require Import Vellvm.Maps Vellvm.Imp.
 Require Import Vellvm.ImpQuickChick.
+
+Require Import Vellvm.CompilerProp Vellvm.Compiler.
 
 Require Import QuickChick.QuickChick.
 Import QcDefaultNotation. Open Scope qc_scope.
@@ -8,16 +10,99 @@ Require Import List ZArith.
 Import ListNotations.
 Require Import String.
 
+Require Import Vellvm.Classes Vellvm.Ollvm_ast.
 
 
 
+Check compile_aexp.
+
+Example empty_ctxt : ctxt := t_empty (None : option Ollvm_ast.value).
+Example test_ctxt :=
+  t_update (t_update empty_ctxt
+                     idX (Some (Ollvm_ast.SV (Ollvm_ast.VALUE_Integer 2%Z))))
+           idY (Some (Ollvm_ast.SV (Ollvm_ast.VALUE_Integer 3%Z))).
+
+Check (compile_aexp empty_ctxt (ANum 2)).
+Compute (compile_aexp empty_ctxt (ANum 2)).
+Compute (compile_aexp empty_ctxt (AId idX)).
+
+Definition test_state := (2, 3, ([]: list elt))%Z.
+Definition test_instr : instr :=
+  INSTR_Op (SV (OP_IBinop (Add false false)
+                          i64
+                          (SV (VALUE_Integer 2%Z))
+                          (SV (VALUE_Integer 2%Z)))).
+
+Definition test_compiled_aexp := compile_aexp test_ctxt (APlus (AId idX) (ANum 3)).
+
+Check fold_left.
+
+(*
+Definition compile (c:com) : err (toplevel_entities (list block)) :=
+  '(fvs, elts) <-
+          run (
+            let fvs := IDSet.elements (fv c) in
+            'g <- compile_fv fvs;  
+(*            '; compile_com g c; *)
+(*            '; print_fv fvs g;  (* UNCOMMENT to enable imp state printing *) *)
+            '; term TERM_Ret_void;    
+            mret fvs
+          );
+  'blocks <- blocks_of_elts (Anon 0)%Z elts;
+  mret
+   ((List.map (fun x => let 'Id s := x in TLE_Declaration (print_decl ("print_" ++ s))) fvs) ++
+   [
+    TLE_Definition
+    {|
+    df_prototype := imp_decl;
+    df_args := [];
+    df_instrs := blocks
+  |}]).
+
+Print toplevel_entity.
+
+Definition ctxt_generator := 
+*)
+                                                
 
 (* Example program that fails imp_compiler_correct here:
 Eample prog1 := X ::= APlus (AId W) (AId W).
-*)
+ *)
+
+Example prog1 := (X ::= ANum 1).
+Example prog2 := (W ::= AId W).
+Example prog3 := X ::= APlus (AId W) (AId W).
+Example prog4 := X ::= APlus (AId W) (AId X). (* fails compilation because not VALUE_Integer *)
+
+Eval vm_compute in (compile prog2).
+
+Definition show_aexp_compilation_result (result : err (value * list elt)) :=
+  match result with
+  | inl _ => "err" 
+  | inr (_, elts) => string_of elts
+  end.
+
+Check (compile prog4).
+
+Definition show_result (result : err (toplevel_entities (list block))) :=
+  match result with
+  | inl _ => "error"
+  | inr l => fold_left (fun s tle_blk => (s ++ "; " ++ (string_of tle_blk))%string) l ""
+  end.
+
+Compute (show_aexp_compilation_result
+           (compile_aexp_wrapper (AMult (AId idX) (APlus (ANum 1) (ANum 2))))).
+
+Compute (show_result (compile prog4)).
+
 
 QuickChick (forAll arbitrary
                    imp_compiler_correct_aux).
+
+
+
+Compute (imp_compiler_correct_aux prog1).
+
 
 
 Definition result1 := imp_compiler_correct_aux prog1.
